Update end-to-end parse table generation function and correctness proofs

LL1/Proofs/ParseTableGen/EndToEnd.v
@@ -1,36 +1,54 @@
+Require Import Lib.Grammar.
+
 Require Import LL1.ParseTableGen.
 Require Import LL1.ParseTable.
 
 Require Import LL1.Proofs.ParseTableGen.mkNullableSet_Correctness.
 Require Import LL1.Proofs.ParseTableGen.mkFirstMap_Correctness.
+Require Import LL1.Proofs.ParseTableGen.mkFollowMap_Correctness.
 Require Import LL1.Proofs.ParseTableGen.mkEntries_Correctness.
 Require Import LL1.Proofs.ParseTableGen.mkParseTable_Correctness.
 
-Theorem genTableForGrammar_sound : 
-  forall g fo tbl,
-  follow_map_for fo g
-  -> genTableForGrammar g fo = Some tbl
+(* Combining all of the steps into a single function *)
+
+Definition parseTableOf (g : grammar) : option parse_table :=
+  let nu := mkNullableSet g in
+  let nu_pf := (mkNullableSet_correct g) in
+  let fi := mkFirstMap g nu in
+  let fi_pf := (mkFirstMap_correct g nu nu_pf) in
+  let fo := mkFollowMap g nu fi fi_pf in
+  let es := mkEntries nu fi fo g in
+  mkParseTable es.
+
+Theorem parseTableOf_sound : 
+  forall g tbl,
+  parseTableOf g = Some tbl
   -> parse_table_for tbl g.
 Proof.
-  intros g fo tbl Hfo Hmk.
+  intros g tbl Hf.
   eapply mkParseTable_sound; eauto.
-  pose proof (mkNullableSet_correct g).
   eapply mkEntries_correct; eauto.
-  apply mkFirstMap_correct; auto.
+  - apply mkNullableSet_correct; auto.
+  - apply mkFirstMap_correct.
+    apply mkNullableSet_correct; auto.
+  - apply mkFollowMap_correct; auto.
+    apply mkNullableSet_correct; auto.
 Qed.
 
-Theorem genTableForGrammar_complete :
-  forall g fo tbl,
-    follow_map_for fo g
-    -> parse_table_for tbl g
+Theorem parseTableOf_complete :
+  forall g tbl,
+    parse_table_for tbl g
     -> exists tbl',
-        ParseTable.Equal tbl tbl'
-        /\ genTableForGrammar g fo = Some tbl'.
+      ParseTable.Equal tbl tbl'
+      /\ parseTableOf g = Some tbl'.
 Proof.
-  intros g fo tbl Hfo Hpt.
+  intros g tbl Hpt.
   eapply mkParseTable_complete; eauto.
-  pose proof (mkNullableSet_correct g).
   eapply mkEntries_correct; eauto.
-  apply mkFirstMap_correct; auto.
+  - apply mkNullableSet_correct; auto.
+  - apply mkFirstMap_correct.
+    apply mkNullableSet_correct; auto.
+  - apply mkFollowMap_correct; auto.
+    apply mkNullableSet_correct; auto.
 Qed.
 
